Project/Basic.lean
@@ -1,0 +1,13 @@
+module
+
+import Mathlib.Computability.Primrec.Basic
+
+@[expose] public section
+
+/--
+Convert a decidable predicate `α → Prop` into an indicator function `α → ℕ`.
+-/
+def ofPred {α} (p : α → Prop) [DecidablePred p] : α → ℕ :=
+  fun a => (decide (p a)).toNat
+
+end
